Done!

ulib/LowStar.Buffer.fst
@@ -64,6 +64,9 @@ let len #a b =
   | Null -> 0ul
   | Buffer _ _ _ len -> len
 
+let live_buffers_same_region_same_address_same_type t1 b1 t2 b2 h =
+  let s0 = (HS.sel h (Buffer?.content b1)) in ()
+
 let len_null a = ()
 
 let lseq (a: Type) (l: nat) : Type =
@@ -412,17 +415,6 @@ let upd #a b i v =
   // prove modifies_1_preserves_abuffers
   Heap.lemma_distinct_addrs_distinct_preorders ();
   Heap.lemma_distinct_addrs_distinct_mm ()
-
-let live_buffers_same_region_same_address_same_type
-  (t1: Type)
-  (b1: buffer t1)
-  (t2: Type)
-  (b2: buffer t2)
-  (h: HS.mem)
-: Lemma
-  (requires ((live h b1 /\ live h b2 /\ frameOf b1 == frameOf b2 /\ as_addr b1 == as_addr b2 /\ length b1 > 0)))
-  (ensures (t1 == t2))
-= let s0 = lseq_of_vec (HS.sel h (Buffer?.content b1)) in ()
 
 (* Recall *)
 
